Examples/EventB/Courses/M1.lean
@@ -1,0 +1,401 @@
+
+import Examples.EventB.Courses.M0
+
+namespace CoursesSpec
+
+structure MembersCtx where
+  members : Finset Member
+
+structure ParticipantsCtx extends MembersCtx where
+  participants : Finset Member
+  parts_prop : participants ⊆ members
+
+structure InstructorsCtx extends M0.Context, MembersCtx where
+  instructors : Finset Member
+  instr_mem_prop : instructors ⊆ members
+  instr_fun : Course → Member
+  intr_fun_prop : ∀ c, c ∈ availableCourses → instr_fun c ∈ instructors
+
+structure M1.Context extends ParticipantsCtx, InstructorsCtx
+
+structure M1 (ctx : M1.Context) extends M0 ctx.toContext where
+  inscriptions : Finset (Course × Member)
+
+/-
+theorem M1.ctx₁ (_ : M1 ctx):
+  ctx.maxOpenedCourses > 0 :=
+by
+  cases ctx.toContext ; simp [*]
+
+theorem M1.ctx₂ (_ : M1 ctx):
+  ctx.maxOpenedCourses ≤ ctx.availableCourses.card :=
+by
+  cases ctx.toContext ; simp [*]
+
+-/
+
+def M1.invariant₁ (m : M1 ctx) : Prop :=
+  m.inscriptions ⊆ m.openedCourses ×ˢ ctx.participants
+
+theorem M1.invariants₁' (m : M1 ctx):
+  m.invariant₁ →
+  ∀ i ∈ m.inscriptions, i.1 ∈ m.openedCourses ∧ i.2 ∈ ctx.participants :=
+by
+  simp [invariant₁]
+  intros Hinv₁ c p
+  intro Hins
+  have Hcp: (c, p) ∈ m.openedCourses ×ˢ ctx.participants := by
+    exact Hinv₁ Hins
+  apply Finset.mem_product (p:=(c, p)).1
+  assumption
+
+def M1.invariant₂ (m : M1 ctx) : Prop :=
+  ∀ i ∈ m.inscriptions, ctx.instr_fun i.1 ≠ i.2
+
+def M1.reset : M1 ctx :=
+  let m0 := M0.reset ctx.toContext
+  { m0 with inscriptions := ∅ }
+
+instance: Machine M1.Context (M1 ctx) where
+  context := ctx
+  invariant m := M0.invariant₁ m.toM0 ∧ M0.invariant₂ m.toM0
+                 ∧ M1.invariant₁ m ∧ M1.invariant₂ m
+  reset := M1.reset
+
+@[simp]
+def M1.lift (m : M1 ctx) : M0 ctx.toContext :=
+  ⟨m.openedCourses⟩
+
+theorem M1.lift_safe (m : M1 ctx):
+  Machine.invariant m → Machine.invariant (M1.lift m) :=
+by
+  simp [Machine.invariant]
+  intros Hinv₁ Hinv₂ _ _
+  constructor
+  case left =>
+    simp [M0.invariant₁]
+    simp [M1.invariant₁, M0.invariant₁] at Hinv₁
+    assumption
+  case right =>
+    simp [M0.invariant₂]
+    simp [M1.invariant₂, M0.invariant₂] at Hinv₂
+    assumption
+
+
+@[simp]
+def M1.unlift (m1 : M1 ctx) (m0' : M0 ctx.toContext) : M1 ctx:=
+  { m0' with inscriptions := m1.inscriptions}
+
+-- this is an interesting property : the abstract machine can move almost "freely"
+theorem M1.unlift_safe (m1 : M1 ctx) (m0 : M0 ctx.toContext):
+  m1.openedCourses = m0.openedCourses
+  → Machine.invariant m1 → Machine.invariant m0
+  → Machine.invariant (M1.unlift m1 m0) :=
+by
+  simp [Machine.invariant]
+  intros Hcs _ _ Hinv₃ Hinv₄ Hainv₁ Hainv₂
+  constructor
+  · simp [M1.invariant₁, M0.invariant₁] at *
+    assumption
+  · constructor
+    · simp [M1.invariant₂, M0.invariant₂] at *
+      assumption
+    · constructor
+      · simp [M1.invariant₁] at *
+        rw [Hcs] at Hinv₃
+        assumption
+      · simp [M1.invariant₂] at *
+        assumption
+
+/-
+
+TODO
+
+instance: SRefinement (M0 ctx.toContext) (M1 ctx) where
+  refine := defaultRefine M1.lift
+  refine_inv m am := by simp
+                        intros Hinv Hlift
+                        rw [Hlift]
+                        apply M1.lift_safe
+                        assumption
+  refine_uniq m am am' := by simp
+                             intros _ Ham Ham'
+                             rw [Ham, ←Ham']
+  lift := M1.lift
+  lift_ref m := by simp
+
+  unlift := M1.unlift
+  lift_unlift m am' := by simp
+
+namespace M1
+namespace Init
+
+@[local simp]
+def init : M1 ctx :=
+  let m0 : M0 ctx.toContext := M0.Init.init
+  { m0 with inscriptions := ∅}
+
+example: let m1 : M1 ctx := init
+         m1.openedCourses = ∅ := by rfl
+
+theorem PO_safety₁:
+  @invariant₁ ctx init :=
+by
+  simp [M1.invariant₁]
+
+theorem PO_safety₂:
+  @invariant₂ ctx init :=
+by
+  simp [M1.invariant₂]
+
+end Init
+
+def Init : SRInitEvent (M0 ctx.toContext) (M1 ctx) Unit Unit := newSRInitEvent' {
+  init := Init.init
+  safety := by simp [Machine.invariant, M1.Init.PO_safety₁, M1.Init.PO_safety₂]
+               constructor
+               · apply M0.Init.PO_safety₁
+               · apply M0.Init.PO_safety₂
+  abstract := M0.Init
+  strengthening := by simp [M0.Init, newInitEvent']
+  simulation := by rfl
+}
+
+def OpenCourses : SRNDEvent (M0 ctx.toContext) (M1 ctx) Unit Unit :=
+  newAbstractSRNDEvent' {
+    event := M0.OpenCourses.toNDEvent
+    step_inv := fun m1 m1' =>
+      by simp [Machine.invariant, M0.OpenCourses, FRefinement.lift, SRefinement.unlift]
+         intros _ _ Hinv₁ Hinv₂ _ cs _ _ Hact₃ _ Hainv'₁ Hainv'₂
+         constructor
+         · assumption
+         · constructor
+           · assumption
+           · constructor
+             · simp [invariant₁] at *
+               rw [Hact₃]
+               have Hcup: m1.openedCourses ×ˢ ctx.participants ⊆ (m1.openedCourses ∪ cs) ×ˢ ctx.participants := by
+                 apply Finset.product_subset_product_left
+                 · apply Finset.subset_union_left
+               exact Finset.Subset.trans Hinv₁ Hcup
+             · simp [invariant₂] at *
+               assumption
+    event_ok := by simp [M0.OpenCourses]
+  }
+
+namespace CloseCourses
+
+@[local simp]
+def guard (m : M1 ctx) (cs : Finset Course) :=
+  M0.CloseCourses.guard m.toM0 cs
+
+def removeCourses (cs : Finset Course) (is : Finset (Course × Member)) : Finset (Course × Member) :=
+  Finset.filter (fun (c', _) => c' ∉ cs) is
+
+theorem removeCourses_mem (cs : Finset Course) (is : Finset (Course × Member)):
+  ∀ cp, cp ∈ removeCourses cs is → cp ∈ is :=
+by
+  simp [removeCourses]
+  intros _ _ H₁ _
+  assumption
+
+theorem removeCourses_memCourse (cs : Finset Course) (is : Finset (Course × Member)):
+  ∀ cp, cp ∈ removeCourses cs is → cp.1 ∉ cs :=
+by
+  simp [removeCourses]
+
+theorem removeCourses_notmem (cs : Finset Course) (is : Finset (Course × Member)):
+  ∀ cp ∈ is, cp.1 ∉ cs → cp ∈ removeCourses cs is :=
+by
+  simp [removeCourses]
+  intros c p Hcp Hc
+  simp [Hcp, Hc]
+
+@[local simp]
+def action (m : M1 ctx) (cs : Finset Course) : M1 ctx :=
+  let am' : M0 ctx.toContext := M0.CloseCourses.action m.toM0 cs
+  { am' with inscriptions := removeCourses cs m.inscriptions}
+
+theorem PO_safety₁ (m : M1 ctx) (cs : Finset Course):
+  invariant₁ m
+  → invariant₁ (action m cs) :=
+by
+  simp [invariant₁, M0.CloseCourses.guard]
+  intros Hinv₁ cp Hrem
+  simp [removeCourses] at Hrem
+  have Hcp := Hinv₁ Hrem.1
+  apply Finset.mem_product.2
+  constructor
+  · refine Finset.mem_sdiff.mpr ?left.a
+    constructor
+    · apply (Finset.mem_product.1 Hcp).left
+    · exact Hrem.2
+  · apply (Finset.mem_product.1 Hcp).right
+
+theorem PO_safety₂ (cs : Finset Course) (m : M1 ctx):
+  invariant₂ m
+  → invariant₂ (action m cs) :=
+by
+  simp [invariant₂, removeCourses]
+  intros Hinv₂ c p Hrem _
+  apply Hinv₂
+  assumption
+
+
+@[local simp]
+def variant (m : M1 ctx) := M0.CloseCourses.variant m.toM0
+
+theorem PO_convergence (m : M1 ctx) (cs : Finset Course):
+  Machine.invariant m
+  → guard m cs
+  → variant (action m cs) < variant m :=
+by
+  simp [Machine.invariant, -guard]
+  intros _ _ _ _ Hgrd
+  apply M0.CloseCourses.PO_convergence
+  assumption
+
+theorem PO_strengthening (m1 : M1 ctx) (cs : Finset Course):
+  Machine.invariant m1
+    → guard m1 cs
+    → let m0 : M0 ctx.toContext := FRefinement.lift m1
+      M0.CloseCourses.toEvent.guard m0 cs :=
+by
+  simp [FRefinement.lift, M0.CloseCourses, newConvergentEvent]
+
+theorem PO_simulation (m1 : M1 ctx) (cs : Finset Course):
+  Machine.invariant m1
+    → guard m1 cs
+    → let m0 : M0 ctx.toContext := FRefinement.lift m1
+      M0.CloseCourses.toEvent.action m0 cs = FRefinement.lift (action m1 cs) :=
+by
+  simp [FRefinement.lift, M0.CloseCourses, newConvergentEvent]
+
+end CloseCourses
+
+def CloseCourses : SRConvergentEvent Nat (M0 ctx.toContext) (M1 ctx) (Finset Course) (Finset Course):= newSRConvergentEvent {
+  guard := CloseCourses.guard
+  action := CloseCourses.action
+  safety := fun m cs => by intros Hinv _
+                           simp [Machine.invariant] at *
+                           simp [Hinv, CloseCourses.PO_safety₁,
+                                      CloseCourses.PO_safety₂]
+                           constructor
+                           · apply M0.CloseCourses.PO_safety₁ ; simp [Hinv]
+                           · apply M0.CloseCourses.PO_safety₂ ; simp [Hinv]
+  absParam := id
+  abstract := M0.CloseCourses.toEvent
+  variant := CloseCourses.variant
+  convergence := CloseCourses.PO_convergence
+  strengthening := CloseCourses.PO_strengthening
+  simulation := CloseCourses.PO_simulation
+}
+
+namespace Register
+
+@[local simp]
+def unregistered? (is : Finset (Course × Member)) (c : Course) (p : Member)  :=
+  (c, p) ∉ is
+
+@[local simp]
+def guard (m : M1 ctx) (p : Member) (c : Course) :=
+  c ∈ m.openedCourses ∧ p ∈ ctx.participants ∧ ctx.instr_fun c ≠ p
+  ∧  unregistered? m.inscriptions c p
+
+@[local simp]
+def action (m : M1 ctx) (p : Member) (c : Course) : M1 ctx :=
+  { openedCourses := m.openedCourses,
+    inscriptions := insert (c,p) m.inscriptions }
+
+theorem PO_safety₁ (m : M1 ctx) (p : Member) (c : Course) :
+  Machine.invariant m → guard m p c
+  → invariant₁ (action m p c) :=
+by
+  simp [Machine.invariant, M0.invariant₁, M0.invariant₂, invariant₁, invariant₂]
+  intros Hainv₁ _ Hinv₁ _ Hgrd₁ Hgrd₂ _ _
+  apply Finset.insert_subset
+  · have Hc: c ∈ ctx.availableCourses := by exact Hainv₁ Hgrd₁
+    have Hp: p ∈ ctx.participants := by exact Hgrd₂
+    simp [Hc, Hp, Hgrd₁]
+  · assumption
+
+theorem PO_safety₂ (m : M1 ctx) (p : Member) (c : Course) :
+  invariant₂ m → guard m p c
+  → invariant₂ (action m p c) :=
+by
+  simp [Machine.invariant, invariant₂]
+  intros Hinv₂ _ _ Hfun _
+  simp [*]
+  exact fun a b a_1 => Hinv₂ a b a_1
+
+def variant (m : M1 ctx) :=
+  (Finset.card m.openedCourses * Finset.card ctx.participants) - Finset.card m.inscriptions
+
+theorem PO_convergence (m : M1 ctx) (p : Member) (c : Course) :
+  Machine.invariant m
+  → guard m p c
+  → variant (action m p c) < variant m :=
+by
+  simp [Machine.invariant, variant]
+  intros Hainv₁ _ Hinv₁ _ Hgrd₁ Hgrd₂ _ Hgrd₄
+  have Hins: (insert (c, p) m.inscriptions).card = m.inscriptions.card + 1 := by
+    exact Finset.card_insert_of_not_mem Hgrd₄
+  simp [Hins] ; clear Hins
+  simp [invariant₁] at Hinv₁
+  simp [M0.invariant₁] at Hainv₁
+
+  have Hsub: m.inscriptions ⊂ m.openedCourses ×ˢ ctx.participants := by
+    apply (Finset.ssubset_iff_of_subset Hinv₁).2
+    exists (c, p)
+    constructor
+    · exact Finset.mk_mem_product Hgrd₁ Hgrd₂
+    · assumption
+
+  have Hins: m.inscriptions.card < (m.openedCourses ×ˢ ctx.participants).card := by
+    exact Finset.card_lt_card Hsub
+
+  rw [Finset.card_product] at Hins
+
+  apply Nat.sub_lt_sub_left
+  · assumption
+  · simp_arith
+
+theorem PO_simulation (m1 : M1 ctx) (p : Member) (c : Course):
+    Machine.invariant m1
+    → guard m1 p c
+    → let m0 : M0 ctx.toContext := M1.lift m1
+      FRefinement.lift (action m1 p c) = m0 :=
+by
+  simp [FRefinement.lift]
+
+end Register
+
+def Register : SRConvergentEvent Nat (M0 ctx.toContext) (M1 ctx) (Member × Course) (Member × Course) :=
+  newConcreteSREvent {
+    guard := fun m (p,c) => Register.guard m p c
+    action := fun m (p,c) => Register.action m p c
+    safety := fun m (p,c) => by simp [Machine.invariant]
+                                intros Hainv₁ Hainv₂ Hinv₁ Hinv₂ Hgrd
+                                constructor
+                                · simp [Register.action, M0.invariant₁] at *
+                                  exact Hainv₁
+                                · constructor
+                                  · simp [Register.action, M0.invariant₂] at *
+                                    exact Hainv₂
+                                  · constructor
+                                    · apply Register.PO_safety₁
+                                      · simp [Machine.invariant, *]
+                                      · assumption
+                                    · exact Register.PO_safety₂ m p c Hinv₂ Hgrd
+
+
+    variant := Register.variant
+    convergence := fun m (p,c) => Register.PO_convergence m p c
+    simulation := fun m (p,c) => Register.PO_simulation m p c
+  }
+
+end M1
+
+-/
+
+end CoursesSpec
